Expose `new_region_modifies`

ulib/FStar.ModifiesGen.fst
@@ -1094,17 +1094,7 @@ let fresh_frame_modifies #al c h0 h1 =
     (fun r a x ->
       c.same_mreference_aloc_preserved #r #a x h0 h1 (fun _ _ _ -> ()))
 
-let new_region_modifies
-  #al
-  (c: cls al)
-  (m0: HS.mem)
-  (r0: HS.rid)
-: Lemma
-  (requires (HS.is_eternal_region r0 /\ HS.live_region m0 r0))
-  (ensures (
-    let (_, m1) = HS.new_eternal_region m0 r0 None in
-    modifies (loc_none #_ #c) m0 m1
-  ))
+let new_region_modifies #al c m0 r0
 = let (_, m1) = HS.new_eternal_region m0 r0 None in
   modifies_intro_strong #_ #c loc_none m0 m1
     (fun _ -> ())
