ulib/FStar.ModifiesGen.fsti
@@ -775,6 +775,18 @@ val fresh_frame_modifies
   (requires (HS.fresh_frame h0 h1))
   (ensures (modifies #_ #c loc_none h0 h1))
 
+val new_region_modifies
+  (#al: aloc_t)
+  (c: cls al)
+  (m0: HS.mem)
+  (r0: HS.rid)
+: Lemma
+  (requires (HS.is_eternal_region r0 /\ HS.live_region m0 r0))
+  (ensures (
+    let (_, m1) = HS.new_eternal_region m0 r0 None in
+    modifies (loc_none #_ #c) m0 m1
+  ))
+
 val popped_modifies
   (#aloc: aloc_t) (c: cls aloc)
   (h0 h1: HS.mem) : Lemma
